HumanEval24 (#174)

HumanEvalLean/HumanEval24.lean
@@ -1,5 +1,134 @@
-def largest_divisor : Unit :=
-  ()
+/-- Computes the largest divisor in O(sqrt n) via trial divison. -/
+def largestDivisor (n : Nat) : Nat :=
+  go 2
+where
+  go (i : Nat) : Nat :=
+    if h : n < i * i then
+      1
+    else if n % i = 0 then
+      n / i
+    else go (i + 1)
+  termination_by n - i
+  decreasing_by
+    have : i < n := by
+      match i with
+      | 0 => omega
+      | 1 => omega
+      | i + 2 => exact Nat.lt_of_lt_of_le (Nat.lt_mul_self_iff.2 (by omega)) (Nat.not_lt.1 h)
+    omega
+
+example : largestDivisor 3 = 1 := by native_decide
+example : largestDivisor 7 = 1 := by native_decide
+example : largestDivisor 10 = 5 := by native_decide
+example : largestDivisor 100 = 50 := by native_decide
+example : largestDivisor 49 = 7 := by native_decide
+
+inductive LargestDivisorSpec (n : Nat) : Nat → Prop
+  | one : (∀ j, 2 ≤ j → j * j ≤ n → n % j ≠ 0) → LargestDivisorSpec n 1
+  | div {i} : (∀ j, 2 ≤ j → j < i → n % j ≠ 0) → 2 ≤ i → n % i = 0 → LargestDivisorSpec n (n / i)
+
+theorem largestDivisorSpec_go {n i : Nat} (hi : 2 ≤ i)
+    (hi' : ∀ j, 2 ≤ j → j < i → n % j ≠ 0) : LargestDivisorSpec n (largestDivisor.go n i) := by
+  fun_induction largestDivisor.go n i
+  case case1 i hni =>
+    rw [largestDivisor.go, dif_pos hni]
+    apply LargestDivisorSpec.one
+    intro j hj hj'
+    apply hi' _ hj
+    exact Nat.mul_self_lt_mul_self_iff.1 (Nat.lt_of_le_of_lt hj' hni)
+  case case2 i hni hni' =>
+    rw [largestDivisor.go, dif_neg hni, if_pos hni']
+    exact LargestDivisorSpec.div hi' hi hni'
+  case case3 i hni hni' ih =>
+    rw [largestDivisor.go, dif_neg hni, if_neg hni']
+    apply ih (by omega)
+    intro j hj hij
+    by_cases hij' : j = i
+    · exact hij' ▸ hni'
+    · exact hi' _ hj (by omega)
+
+theorem largestDivisorSpec_largestDivisor {n : Nat} :
+    LargestDivisorSpec n (largestDivisor n) := by
+  rw [largestDivisor]
+  exact largestDivisorSpec_go (Nat.le_refl _) (by omega)
+
+theorem Nat.lt_mul_iff {a b : Nat} : a < a * b ↔ 0 < a ∧ 1 < b := by
+  obtain (rfl|ha) := Nat.eq_zero_or_pos a
+  · simp
+  · simp [ha]
+
+theorem helper {n i : Nat} (hn : 1 < n) (h : ∀ j, 2 ≤ j → j < i → n % j ≠ 0) (hi : n % i = 0)
+    (k : Nat) (hk : n / i < k) (hk₁ : k < n) : n % k ≠ 0 := by
+  intro hk₂
+  obtain ⟨d, rfl⟩ := Nat.dvd_of_mod_eq_zero hk₂
+  rw [Nat.lt_mul_iff] at hk₁
+  have hi₀ : 0 < i := by
+    apply Nat.pos_iff_ne_zero.2
+    rintro rfl
+    simp only [Nat.mod_zero] at hi
+    omega
+  refine h d ?_ ?_ (by simp)
+  · omega
+  · rw [Nat.div_lt_iff_lt_mul hi₀] at hk
+    exact Nat.lt_of_mul_lt_mul_left hk
+
+theorem similar_helper {n : Nat} (hn : 1 < n) (h : ∀ j, 2 ≤ j → j * j ≤ n → n % j ≠ 0)
+    (k : Nat) (hk : n < k * k) (hk₁ : k < n) : n % k ≠ 0 := by
+  intro hk₂
+  obtain ⟨d, rfl⟩ := Nat.dvd_of_mod_eq_zero hk₂
+  rw [Nat.lt_mul_iff] at hk₁
+  refine h d ?_ ?_ (by simp)
+  · omega
+  · refine Nat.mul_le_mul_right _ (Nat.le_of_lt ?_)
+    exact Nat.lt_of_mul_lt_mul_left hk
+
+theorem largestDivisorSpec_iff {n i : Nat} (hn : 1 < n) :
+    LargestDivisorSpec n i ↔ i < n ∧ n % i = 0 ∧ ∀ j, j < n → n % j = 0 → j ≤ i := by
+  constructor
+  · rintro (h|h)
+    · refine ⟨hn, Nat.mod_one _, fun j hj hj₁ => Nat.not_lt.1 (fun hj₂ => ?_)⟩
+      by_cases hj₃ : j * j ≤ n
+      · exact h j (by omega) hj₃ hj₁
+      · exact similar_helper hn h j (by omega) hj hj₁
+    · rename_i i hi hi'
+      refine ⟨?_, ?_, fun j hj hj₁ => ?_⟩
+      · apply Nat.div_lt_self <;> omega
+      · exact Nat.mod_eq_zero_of_dvd (Nat.div_dvd_of_dvd (Nat.dvd_of_mod_eq_zero hi'))
+      · exact Nat.not_lt.1 (fun hj₂ => helper hn h hi' j hj₂ hj hj₁)
+  · rintro ⟨hi₁, hi₂, hi₃⟩
+    obtain (h|rfl|h) := Nat.lt_trichotomy i 1
+    · obtain rfl : i = 0 := by omega
+      omega
+    · refine LargestDivisorSpec.one (fun j hj hj₁ hj₂ => absurd (hi₃ j ?_ hj₂) (by omega))
+      exact Nat.lt_of_lt_of_le (Nat.lt_mul_self_iff.2 (by omega)) hj₁
+    · obtain ⟨d, rfl⟩ := Nat.dvd_of_mod_eq_zero hi₂
+      have hd : 0 < d := Nat.pos_iff_ne_zero.2 (fun hd => by simp [hd] at hn)
+      rw (occs := [2]) [← Nat.mul_div_cancel (m := i) (n := d) hd]
+      refine LargestDivisorSpec.div ?_ ?_ (by simp)
+      · intro j hj₁ hj₂ hj₃
+        have : ¬ i * d / j ≤ i := by
+          rw [Nat.not_le, Nat.lt_div_iff_mul_lt_of_dvd (by omega) (Nat.dvd_of_mod_eq_zero hj₃)]
+          exact Nat.mul_lt_mul_of_pos_left hj₂ (by omega)
+        refine absurd (hi₃ _ ?_ ?_) this
+        · apply Nat.div_lt_self (by omega) (by omega)
+        · exact Nat.mod_eq_zero_of_dvd (Nat.div_dvd_of_dvd (Nat.dvd_of_mod_eq_zero hj₃))
+      · rw [Nat.lt_mul_iff] at hi₁
+        omega
+
+theorem largestDivisorSpec_unique {n i k : Nat} (hn : 1 < n)
+    (hi : LargestDivisorSpec n i) (hk : LargestDivisorSpec n k) : i = k := by
+  simp only [largestDivisorSpec_iff hn] at hi hk
+  apply Nat.le_antisymm
+  · apply hk.2.2 _ hi.1 hi.2.1
+  · apply hi.2.2 _ hk.1 hk.2.1
+
+theorem largestDivisor_eq_iff {n i : Nat} (hn : 1 < n) :
+    largestDivisor n = i ↔ i < n ∧ n % i = 0 ∧ ∀ j, j < n → n % j = 0 → j ≤ i := by
+  rw [← largestDivisorSpec_iff hn]
+  refine ⟨?_, fun hi => ?_⟩
+  · rintro rfl
+    apply largestDivisorSpec_largestDivisor
+  · apply largestDivisorSpec_unique hn largestDivisorSpec_largestDivisor hi
 
 /-!
 ## Prompt
